projection/proofs/endpointConfluenceScript.sml
@@ -1,0 +1,1653 @@
+open preamble endpointSemanticsTheory endpointLangTheory endpointPropsTheory;
+
+val _ = new_theory "endpointConfluence";
+
+Theorem endpoint_local_confluence_send:
+  ∀p1 alpha p2 p3 s d r.
+  trans p1 alpha p2 /\ trans p1 (LSend s d r) p3 /\ p2 <> p3 /\
+  ALL_DISTINCT (MAP FST (endpoints p1)) /\
+  ~MEM r (MAP FST (endpoints p1))
+  ==>
+  ?p4 p5. trans p2 (LSend s d r) p4 /\
+        trans p3 alpha p4
+Proof
+  simp[GSYM AND_IMP_INTRO, GSYM PULL_FORALL]
+  >> ho_match_mp_tac trans_strongind
+  >> rpt strip_tac >> fs[] >> rveq
+  >- (* Send *)
+     (qhdtm_x_assum `trans` (assume_tac o SIMP_RULE std_ss [Once trans_cases]) >>
+      fs[] >> rveq >> fs[] >> rveq >> fs[])
+  >- (* Enqueue *)
+      (qhdtm_x_assum `trans` (assume_tac o SIMP_RULE std_ss [Once trans_cases]) >>
+       fs[] >> rveq >> fs[] >> rveq >> fs[]
+       >- (qmatch_goalsub_abbrev_tac `NEndpoint _ s1` >>
+           rename1 `FLOOKUP s.bindings v = SOME data` >>
+           `FLOOKUP s1.bindings v = SOME data` by simp[Abbr`s1`] >>
+           drule trans_send >> simp[] >>
+           disch_then dxrule >>
+           rename1 `Send _ _ e1` >>
+           disch_then(qspec_then `e1` assume_tac) >>
+           asm_exists_tac >> simp[] >>
+           drule trans_enqueue >>
+           metis_tac[])
+       >- (qmatch_goalsub_abbrev_tac `NEndpoint _ s1` >>
+           rename1 `FLOOKUP s.bindings v = SOME data` >>
+           `FLOOKUP s1.bindings v = SOME data` by simp[Abbr`s1`] >>
+           drule trans_send >> simp[] >>
+           disch_then dxrule >>
+           rename1 `Send _ _ e1` >>
+           disch_then(qspec_then `e1` assume_tac) >>
+           asm_exists_tac >> simp[] >>
+           drule trans_enqueue >>
+           metis_tac[]))
+  >- (* Com-L *)
+     (qhdtm_x_assum `trans` (assume_tac o SIMP_RULE std_ss [Once trans_cases]) >>
+      fs[] >> rveq >> fs[] >> rveq >> fs[]
+      >- (fs[endpoints_def,ALL_DISTINCT_APPEND] >>
+          first_x_assum(drule_all_then strip_assume_tac) >>
+          metis_tac[trans_com_l,trans_par_l])
+      >- (fs[endpoints_def,ALL_DISTINCT_APPEND] >>
+          first_x_assum drule >>
+          imp_res_tac sender_is_endpoint >>
+          imp_res_tac receiver_is_endpoint >>
+          Cases_on `s = p1''` (* TODO: generated names *)
+          >- metis_tac[trans_same_sender_determ] >>
+          drule_then assume_tac (GEN_ALL trans_different_sender) >>
+          qpat_x_assum `trans _ (LSend _ _ _) _` mp_tac >>
+          pop_assum drule >> impl_tac >- simp[] >>
+          ntac 2 strip_tac >> impl_tac >- simp[] >>
+          strip_tac >> metis_tac[trans_par_l,trans_com_l])
+      >- (fs[endpoints_def,ALL_DISTINCT_APPEND] >>
+          first_x_assum drule >>
+          imp_res_tac sender_is_endpoint >>
+          imp_res_tac receiver_is_endpoint >>
+          impl_tac >- metis_tac[trans_send_receive_distinct] >>
+          strip_tac >> metis_tac[trans_par_r,trans_com_l])
+      >- (fs[endpoints_def,ALL_DISTINCT_APPEND] >>
+          first_x_assum drule >>
+          imp_res_tac sender_is_endpoint >>
+          imp_res_tac receiver_is_endpoint >>
+          impl_tac >- metis_tac[trans_send_receive_distinct] >>
+          strip_tac >> metis_tac[trans_par_r,trans_com_l]))
+  >- (* Com-R *)
+     (qhdtm_x_assum `trans` (assume_tac o SIMP_RULE std_ss [Once trans_cases]) >>
+      fs[] >> rveq >> fs[] >> rveq >> fs[]
+      >- (fs[endpoints_def,ALL_DISTINCT_APPEND] >>
+          first_x_assum(drule_all_then strip_assume_tac) >>
+          metis_tac[trans_com_r,trans_par_l])
+      >- (fs[endpoints_def,ALL_DISTINCT_APPEND] >>
+          last_x_assum drule >>
+          imp_res_tac sender_is_endpoint >>
+          imp_res_tac receiver_is_endpoint >>
+          impl_tac >- metis_tac[trans_send_receive_distinct] >>
+          strip_tac >> metis_tac[trans_par_l,trans_com_r])
+      >- (fs[endpoints_def,ALL_DISTINCT_APPEND] >>
+          last_x_assum drule >>
+          imp_res_tac sender_is_endpoint >>
+          imp_res_tac receiver_is_endpoint >>
+          Cases_on `s = p1''` (* TODO: generated names *)
+          >- metis_tac[trans_same_sender_determ] >>
+          drule_then assume_tac (GEN_ALL trans_different_sender) >>
+          qpat_x_assum `trans _ (LSend _ _ _) _` mp_tac >>
+          pop_assum drule >> impl_tac >- simp[] >>
+          ntac 2 strip_tac >> impl_tac >- simp[] >>
+          strip_tac >> metis_tac[trans_par_r,trans_com_r])
+      >- (fs[endpoints_def,ALL_DISTINCT_APPEND] >>
+          last_x_assum drule >>
+          imp_res_tac sender_is_endpoint >>
+          imp_res_tac receiver_is_endpoint >>
+          impl_tac >- metis_tac[trans_send_receive_distinct] >>
+          strip_tac >> metis_tac[trans_par_r,trans_com_r]))
+  >- (* IntChoice *)
+     (qhdtm_x_assum `trans` (assume_tac o SIMP_RULE std_ss [Once trans_cases]) >>
+      fs[] >> rveq >> fs[] >> rveq >> fs[])
+  >- (* Enqueue-Choice-L *)
+     (qhdtm_x_assum `trans` (assume_tac o SIMP_RULE std_ss [Once trans_cases]) >>
+      fs[] >> rveq >> fs[] >> rveq >> fs[] >>
+      fs[endpoints_def] >>
+      qmatch_goalsub_abbrev_tac `trans (NEndpoint p2 s1 (Send r v e))` >>
+      qexists_tac `NEndpoint p2 s1 e` >>
+      TRY(conj_tac
+          >- (match_mp_tac trans_send >> simp[Abbr `s1`])
+          >- metis_tac[trans_enqueue_choice_l]))
+  >- (* Enqueue-Choice-R *)
+     (qhdtm_x_assum `trans` (assume_tac o SIMP_RULE std_ss [Once trans_cases]) >>
+      fs[] >> rveq >> fs[] >> rveq >> fs[] >>
+      fs[endpoints_def] >>
+      qmatch_goalsub_abbrev_tac `trans (NEndpoint p2 s1 (Send r v e))` >>
+      qexists_tac `NEndpoint p2 s1 e` >>
+      TRY(conj_tac
+          >- (match_mp_tac trans_send >> simp[Abbr `s1`])
+          >- metis_tac[trans_enqueue_choice_r]))
+  >- (* Com-Choice-L *)
+     (qhdtm_x_assum `trans` (assume_tac o SIMP_RULE std_ss [Once trans_cases]) >>
+      fs[] >> rveq >> fs[] >> rveq >> fs[]
+      >- (fs[endpoints_def,ALL_DISTINCT_APPEND] >>
+          first_x_assum(drule_all_then strip_assume_tac) >>
+          metis_tac[trans_com_choice_l,trans_par_l])
+      >- (fs[endpoints_def,ALL_DISTINCT_APPEND] >>
+          first_x_assum drule >>
+          imp_res_tac sender_is_endpoint >>
+          imp_res_tac receiver_is_endpoint >>
+          drule(GEN_ALL trans_send_choice_distinct_senders) >>
+          disch_then drule >>
+          impl_tac >- simp[] >>
+          strip_tac >>
+          dxrule trans_distinct_residual >>
+          disch_then drule >>
+          impl_tac >- simp[label_rel_def,receive_ext_choice_rel_def] >>
+          strip_tac >>
+          impl_tac >- simp[] >>
+          strip_tac >>
+          metis_tac[trans_par_l,trans_com_choice_l])
+      >- (fs[endpoints_def,ALL_DISTINCT_APPEND] >>
+          first_x_assum drule >>
+          imp_res_tac sender_is_endpoint >>
+          imp_res_tac receiver_is_endpoint >>
+          dxrule trans_distinct_residual >>
+          disch_then drule >>
+          impl_tac >- simp[label_rel_def,receive_ext_choice_rel_def] >>
+          strip_tac >>
+          impl_tac >- simp[] >>
+          strip_tac >>
+          metis_tac[trans_par_r,trans_com_choice_l])
+      >- (fs[endpoints_def,ALL_DISTINCT_APPEND] >>
+          first_x_assum drule >>
+          imp_res_tac sender_is_endpoint >>
+          imp_res_tac receiver_is_endpoint >>
+          dxrule trans_distinct_residual >>
+          disch_then drule >>
+          impl_tac >- simp[label_rel_def,receive_ext_choice_rel_def] >>
+          strip_tac >>
+          impl_tac >- simp[] >>
+          metis_tac[trans_par_r,trans_com_choice_l]))
+  >- (* Com-Choice-R *)
+     (qhdtm_x_assum `trans` (assume_tac o SIMP_RULE std_ss [Once trans_cases]) >>
+      fs[] >> rveq >> fs[] >> rveq >> fs[]
+      >- (fs[endpoints_def,ALL_DISTINCT_APPEND] >>
+          first_x_assum(drule_all_then strip_assume_tac) >>
+          metis_tac[trans_com_choice_r,trans_par_l])
+      >- (fs[endpoints_def,ALL_DISTINCT_APPEND] >>
+          last_x_assum drule >>
+          imp_res_tac sender_is_endpoint >>
+          imp_res_tac receiver_is_endpoint >>
+          dxrule(GEN_ALL trans_distinct_residual) >>
+          disch_then drule >>
+          impl_tac >- simp[label_rel_def,receive_ext_choice_rel_def] >>
+          strip_tac >>
+          impl_tac >- simp[] >>
+          metis_tac[trans_par_l,trans_com_choice_r])
+      >- (fs[endpoints_def,ALL_DISTINCT_APPEND] >>
+          first_x_assum drule >>
+          imp_res_tac sender_is_endpoint >>
+          imp_res_tac receiver_is_endpoint >>
+          dxrule trans_distinct_residual >>
+          disch_then drule >>
+          impl_tac >- simp[label_rel_def,receive_ext_choice_rel_def] >>
+          strip_tac >>
+          impl_tac >- simp[] >>
+          strip_tac >>
+          metis_tac[trans_par_r,trans_com_choice_r])
+      >- (fs[endpoints_def,ALL_DISTINCT_APPEND] >>
+          first_x_assum drule >>
+          imp_res_tac sender_is_endpoint >>
+          imp_res_tac receiver_is_endpoint >>
+          dxrule trans_distinct_residual >>
+          disch_then drule >>
+          impl_tac >- simp[label_rel_def,receive_ext_choice_rel_def] >>
+          strip_tac >>
+          impl_tac >- simp[] >>
+          metis_tac[trans_par_r,trans_com_choice_r]))
+  >- (* Dequeue *)
+     (qhdtm_x_assum `trans` (assume_tac o SIMP_RULE std_ss [Once trans_cases]) >>
+      fs[] >> rveq >> fs[] >> rveq >> fs[])
+  >- (* ExtChoice-L *)
+     (qhdtm_x_assum `trans` (assume_tac o SIMP_RULE std_ss [Once trans_cases]) >>
+      fs[] >> rveq >> fs[] >> rveq >> fs[])
+  >- (* ExtChoice-R *)
+     (qhdtm_x_assum `trans` (assume_tac o SIMP_RULE std_ss [Once trans_cases]) >>
+      fs[] >> rveq >> fs[] >> rveq >> fs[])
+  >- (* If-L *)
+     (qhdtm_x_assum `trans` (assume_tac o SIMP_RULE std_ss [Once trans_cases]) >>
+      fs[] >> rveq >> fs[] >> rveq >> fs[])
+  >- (* If-R *)
+     (qhdtm_x_assum `trans` (assume_tac o SIMP_RULE std_ss [Once trans_cases]) >>
+      fs[] >> rveq >> fs[] >> rveq >> fs[])
+  >- (* Let *)
+     (qhdtm_x_assum `trans` (assume_tac o SIMP_RULE std_ss [Once trans_cases]) >>
+      fs[] >> rveq >> fs[] >> rveq >> fs[])
+  >- (* Par-L *)
+     (qhdtm_x_assum `trans` (assume_tac o SIMP_RULE std_ss [Once trans_cases]) >>
+      fs[] >> rveq >> fs[] >> rveq >> fs[]
+      >- (fs[endpoints_def,ALL_DISTINCT_APPEND] >>
+          metis_tac[trans_par_l])
+      >- (metis_tac[trans_par_l,trans_par_r])
+      >- (metis_tac[trans_par_l,trans_par_r]))
+  >- (* Par-R *)
+     (qhdtm_x_assum `trans` (assume_tac o SIMP_RULE std_ss [Once trans_cases]) >>
+      fs[] >> rveq >> fs[] >> rveq >> fs[]
+      >- metis_tac[trans_par_l,trans_par_r] >>
+      fs[endpoints_def,ALL_DISTINCT_APPEND] >>
+      metis_tac[trans_par_r,trans_par_l])
+QED
+
+Theorem endpoint_local_confluence_send_rotated:
+  ∀p1 alpha p2 p3 s d r.
+  trans p1 (LSend s d r) p3 /\ trans p1 alpha p2 /\ p2 <> p3 /\
+  ALL_DISTINCT (MAP FST (endpoints p1)) /\
+  ~MEM r (MAP FST (endpoints p1))
+  ==>
+  ?p4 p5. trans p2 (LSend s d r) p4 /\
+        trans p3 alpha p4
+Proof
+  metis_tac[endpoint_local_confluence_send]
+QED
+
+Theorem endpoint_local_confluence_int_choice:
+  ∀p1 alpha p2 p3 s b r.
+  trans p1 alpha p2 /\ trans p1 (LIntChoice s b r) p3 /\ p2 <> p3 /\
+  ALL_DISTINCT (MAP FST (endpoints p1)) /\
+  ~MEM r (MAP FST (endpoints p1))
+  ==>
+  ?p4 p5. trans p2 (LIntChoice s b r) p4 /\
+        trans p3 alpha p4
+Proof
+  simp[GSYM AND_IMP_INTRO, GSYM PULL_FORALL]
+  >> ho_match_mp_tac trans_strongind
+  >> rpt strip_tac >> fs[] >> rveq
+  >- (* Send *)
+     (qhdtm_x_assum `trans` (assume_tac o SIMP_RULE std_ss [Once trans_cases]) >>
+      fs[] >> rveq >> fs[] >> rveq >> fs[])
+  >- (* Enqueue *)
+      (qhdtm_x_assum `trans` (assume_tac o SIMP_RULE std_ss [Once trans_cases]) >>
+       fs[] >> rveq >> fs[] >> rveq >> fs[]
+       >- (qmatch_goalsub_abbrev_tac `NEndpoint _ s1` >>
+           dxrule trans_int_choice >>
+           rename1 `IntChoice _ _ e1` >>
+           disch_then(qspecl_then [`s1`,`b`,`e1`] assume_tac) >>
+           asm_exists_tac >> simp[] >>
+           drule trans_enqueue >>
+           metis_tac[])
+       >- (qmatch_goalsub_abbrev_tac `NEndpoint _ s1` >>
+           dxrule trans_int_choice >> simp[] >>
+           rename1 `IntChoice _ _ e1` >>
+           disch_then(qspecl_then [`s1`,`b`,`e1`] assume_tac) >>
+           asm_exists_tac >> simp[] >>
+           drule trans_enqueue >>
+           metis_tac[]))
+  >- (* Com-L *)
+     (qhdtm_x_assum `trans` (assume_tac o SIMP_RULE std_ss [Once trans_cases]) >>
+      fs[] >> rveq >> fs[] >> rveq >> fs[]
+      >- (fs[endpoints_def,ALL_DISTINCT_APPEND] >>
+          first_x_assum(drule_all_then strip_assume_tac) >>
+          metis_tac[trans_com_l,trans_par_l])
+      >- (fs[endpoints_def,ALL_DISTINCT_APPEND] >>
+          first_x_assum drule >>
+          imp_res_tac sender_is_endpoint >>
+          imp_res_tac receiver_is_endpoint >>
+          imp_res_tac choice_sender_is_endpoint >>
+          dxrule trans_distinct_residual >>
+          disch_then dxrule >>
+          impl_tac >- simp[label_rel_def,receive_ext_choice_rel_def] >>
+          strip_tac >>
+          impl_tac >- simp[] >>
+          strip_tac >>
+          metis_tac[trans_par_l,trans_com_l])
+      >- (fs[endpoints_def,ALL_DISTINCT_APPEND] >>
+          first_x_assum drule >>
+          imp_res_tac sender_is_endpoint >>
+          imp_res_tac receiver_is_endpoint >>
+          imp_res_tac choice_sender_is_endpoint >>
+          dxrule trans_distinct_residual >>
+          disch_then dxrule >>
+          impl_tac >- simp[label_rel_def,receive_ext_choice_rel_def] >>
+          strip_tac >>
+          impl_tac >- metis_tac[trans_send_receive_distinct] >>
+          strip_tac >> metis_tac[trans_par_r,trans_com_l])
+      >- (fs[endpoints_def,ALL_DISTINCT_APPEND] >>
+          first_x_assum drule >>
+          imp_res_tac sender_is_endpoint >>
+          imp_res_tac receiver_is_endpoint >>
+          imp_res_tac choice_sender_is_endpoint >>
+          impl_tac >- metis_tac[trans_send_receive_distinct] >>
+          strip_tac >> metis_tac[trans_par_r,trans_com_l]))
+  >- (* Com-R *)
+     (qhdtm_x_assum `trans` (assume_tac o SIMP_RULE std_ss [Once trans_cases]) >>
+      fs[] >> rveq >> fs[] >> rveq >> fs[]
+      >- (fs[endpoints_def,ALL_DISTINCT_APPEND] >>
+          first_x_assum(drule_all_then strip_assume_tac) >>
+          metis_tac[trans_com_r,trans_par_l])
+      >- (fs[endpoints_def,ALL_DISTINCT_APPEND] >>
+          last_x_assum drule >>
+          imp_res_tac sender_is_endpoint >>
+          imp_res_tac receiver_is_endpoint >>
+          imp_res_tac choice_sender_is_endpoint >>
+          dxrule trans_distinct_residual >>
+          disch_then dxrule >>
+          impl_tac >- simp[label_rel_def,receive_ext_choice_rel_def] >>
+          strip_tac >>
+          impl_tac >- metis_tac[trans_send_receive_distinct] >>
+          strip_tac >> metis_tac[trans_par_l,trans_com_r])
+      >- (fs[endpoints_def,ALL_DISTINCT_APPEND] >>
+          last_x_assum drule >>
+          imp_res_tac sender_is_endpoint >>
+          imp_res_tac receiver_is_endpoint >>
+          imp_res_tac choice_sender_is_endpoint >>
+          dxrule trans_distinct_residual >>
+          disch_then dxrule >>
+          impl_tac >- simp[label_rel_def,receive_ext_choice_rel_def] >>
+          strip_tac >>
+          impl_tac >- simp[] >>
+          strip_tac >> metis_tac[trans_par_r,trans_com_r])
+      >- (fs[endpoints_def,ALL_DISTINCT_APPEND] >>
+          last_x_assum drule >>
+          imp_res_tac sender_is_endpoint >>
+          imp_res_tac receiver_is_endpoint >>
+          imp_res_tac choice_sender_is_endpoint >>
+          impl_tac >- metis_tac[trans_send_receive_distinct] >>
+          strip_tac >> metis_tac[trans_par_r,trans_com_r]))
+  >- (* IntChoice *)
+     (qhdtm_x_assum `trans` (assume_tac o SIMP_RULE std_ss [Once trans_cases]) >>
+      fs[] >> rveq >> fs[] >> rveq >> fs[])
+  >- (* Enqueue-Choice-L *)
+     (qhdtm_x_assum `trans` (assume_tac o SIMP_RULE std_ss [Once trans_cases]) >>
+      fs[] >> rveq >> fs[] >> rveq >> fs[] >>
+      fs[endpoints_def] >>
+      qmatch_goalsub_abbrev_tac `trans (NEndpoint p2 s1 (IntChoice b r e))` >>
+      qexists_tac `NEndpoint p2 s1 e` >>
+      TRY(conj_tac
+          >- (match_mp_tac trans_int_choice >> simp[Abbr `s1`])
+          >- metis_tac[trans_enqueue_choice_l]))
+  >- (* Enqueue-Choice-R *)
+     (qhdtm_x_assum `trans` (assume_tac o SIMP_RULE std_ss [Once trans_cases]) >>
+      fs[] >> rveq >> fs[] >> rveq >> fs[] >>
+      fs[endpoints_def] >>
+      qmatch_goalsub_abbrev_tac `trans (NEndpoint p2 s1 (IntChoice b r e))` >>
+      qexists_tac `NEndpoint p2 s1 e` >>
+      TRY(conj_tac
+          >- (match_mp_tac trans_int_choice >> simp[Abbr `s1`])
+          >- metis_tac[trans_enqueue_choice_r]))
+  >- (* Com-Choice-L *)
+     (qhdtm_x_assum `trans` (assume_tac o SIMP_RULE std_ss [Once trans_cases]) >>
+      fs[] >> rveq >> fs[] >> rveq >> fs[]
+      >- (fs[endpoints_def,ALL_DISTINCT_APPEND] >>
+          first_x_assum(drule_all_then strip_assume_tac) >>
+          metis_tac[trans_com_choice_l,trans_par_l])
+      >- (fs[endpoints_def,ALL_DISTINCT_APPEND] >>
+          first_x_assum drule >>
+          Cases_on `p1'' = s` (* TODO: generated names *)
+          >- (rveq >>
+              imp_res_tac choice_sender_is_endpoint >>
+              imp_res_tac choice_receiver_is_endpoint >>
+              dxrule_all_then strip_assume_tac trans_same_sender_choice_determ >>
+              rveq >> fs[]
+             ) >>
+          imp_res_tac choice_sender_is_endpoint >>
+          imp_res_tac choice_receiver_is_endpoint >>
+          dxrule trans_distinct_residual >>
+          disch_then drule >>
+          impl_tac >- simp[label_rel_def,receive_ext_choice_rel_def] >>
+          strip_tac >>
+          impl_tac >- simp[] >>
+          strip_tac >>
+          metis_tac[trans_par_l,trans_com_choice_l])
+      >- (fs[endpoints_def,ALL_DISTINCT_APPEND] >>
+          first_x_assum drule >>
+          imp_res_tac sender_is_endpoint >>
+          imp_res_tac receiver_is_endpoint >>
+          dxrule trans_distinct_residual >>
+          disch_then drule >>
+          impl_tac >- simp[label_rel_def,receive_ext_choice_rel_def] >>
+          strip_tac >>
+          impl_tac >- simp[] >>
+          strip_tac >>
+          metis_tac[trans_par_r,trans_com_choice_l])
+      >- (fs[endpoints_def,ALL_DISTINCT_APPEND] >>
+          first_x_assum drule >>
+          imp_res_tac sender_is_endpoint >>
+          imp_res_tac receiver_is_endpoint >>
+          dxrule trans_distinct_residual >>
+          disch_then drule >>
+          impl_tac >- simp[label_rel_def,receive_ext_choice_rel_def] >>
+          strip_tac >>
+          impl_tac >- simp[] >>
+          metis_tac[trans_par_r,trans_com_choice_l]))
+  >- (* Com-Choice-R *)
+     (qhdtm_x_assum `trans` (assume_tac o SIMP_RULE std_ss [Once trans_cases]) >>
+      fs[] >> rveq >> fs[] >> rveq >> fs[]
+      >- (fs[endpoints_def,ALL_DISTINCT_APPEND] >>
+          first_x_assum(drule_all_then strip_assume_tac) >>
+          metis_tac[trans_com_choice_r,trans_par_l])
+      >- (fs[endpoints_def,ALL_DISTINCT_APPEND] >>
+          last_x_assum drule >>
+          imp_res_tac sender_is_endpoint >>
+          imp_res_tac receiver_is_endpoint >>
+          dxrule trans_distinct_residual >>
+          disch_then drule >>
+          impl_tac >- simp[label_rel_def,receive_ext_choice_rel_def] >>
+          strip_tac >>
+          impl_tac >- simp[] >>
+          strip_tac >>
+          metis_tac[trans_par_l,trans_com_choice_r])
+      >- (fs[endpoints_def,ALL_DISTINCT_APPEND] >>
+          last_x_assum drule >>
+          imp_res_tac choice_sender_is_endpoint >>
+          imp_res_tac choice_receiver_is_endpoint >>
+          Cases_on `p1'' = s` (* TODO: generated names *)
+          >- (rveq >>
+              dxrule_all_then strip_assume_tac trans_same_sender_choice_determ >>
+              rveq >> fs[]
+             ) >>          
+          dxrule(GEN_ALL trans_distinct_residual) >>
+          disch_then drule >>
+          impl_tac >- simp[label_rel_def,receive_ext_choice_rel_def] >>
+          strip_tac >>
+          impl_tac >- simp[] >>
+          metis_tac[trans_par_r,trans_com_choice_r])
+      >- (fs[endpoints_def,ALL_DISTINCT_APPEND] >>
+          first_x_assum drule >>
+          imp_res_tac choice_sender_is_endpoint >>
+          imp_res_tac choice_receiver_is_endpoint >>
+          Cases_on `p1'' = s` (* TODO: generated names *)
+          >- (rveq >>
+              dxrule_all_then strip_assume_tac trans_same_sender_choice_determ >>
+              rveq >> fs[]
+             ) >>
+          dxrule trans_distinct_residual >>
+          disch_then drule >>
+          impl_tac >- simp[label_rel_def,receive_ext_choice_rel_def] >>
+          strip_tac >>
+          impl_tac >- simp[] >>
+          strip_tac >>
+          metis_tac[trans_par_r,trans_com_choice_r]))
+  >- (* Dequeue *)
+     (qhdtm_x_assum `trans` (assume_tac o SIMP_RULE std_ss [Once trans_cases]) >>
+      fs[] >> rveq >> fs[] >> rveq >> fs[])
+  >- (* ExtChoice-L *)
+     (qhdtm_x_assum `trans` (assume_tac o SIMP_RULE std_ss [Once trans_cases]) >>
+      fs[] >> rveq >> fs[] >> rveq >> fs[])
+  >- (* ExtChoice-R *)
+     (qhdtm_x_assum `trans` (assume_tac o SIMP_RULE std_ss [Once trans_cases]) >>
+      fs[] >> rveq >> fs[] >> rveq >> fs[])
+  >- (* If-L *)
+     (qhdtm_x_assum `trans` (assume_tac o SIMP_RULE std_ss [Once trans_cases]) >>
+      fs[] >> rveq >> fs[] >> rveq >> fs[])
+  >- (* If-R *)
+     (qhdtm_x_assum `trans` (assume_tac o SIMP_RULE std_ss [Once trans_cases]) >>
+      fs[] >> rveq >> fs[] >> rveq >> fs[])
+  >- (* Let *)
+     (qhdtm_x_assum `trans` (assume_tac o SIMP_RULE std_ss [Once trans_cases]) >>
+      fs[] >> rveq >> fs[] >> rveq >> fs[])
+  >- (* Par-L *)
+     (qhdtm_x_assum `trans` (assume_tac o SIMP_RULE std_ss [Once trans_cases]) >>
+      fs[] >> rveq >> fs[] >> rveq >> fs[]
+      >- (fs[endpoints_def,ALL_DISTINCT_APPEND] >>
+          metis_tac[trans_par_l])
+      >- (metis_tac[trans_par_l,trans_par_r])
+      >- (metis_tac[trans_par_l,trans_par_r]))
+  >- (* Par-R *)
+     (qhdtm_x_assum `trans` (assume_tac o SIMP_RULE std_ss [Once trans_cases]) >>
+      fs[] >> rveq >> fs[] >> rveq >> fs[]
+      >- metis_tac[trans_par_l,trans_par_r] >>
+      fs[endpoints_def,ALL_DISTINCT_APPEND] >>
+      metis_tac[trans_par_r,trans_par_l])
+QED
+
+Theorem endpoint_local_confluence_int_choice_rotated:
+  ∀p1 alpha p2 p3 s b r.
+  trans p1 (LIntChoice s b r) p3 /\ trans p1 alpha p2 /\ p2 <> p3 /\
+  ALL_DISTINCT (MAP FST (endpoints p1)) /\
+  ~MEM r (MAP FST (endpoints p1))
+  ==>
+  ?p4 p5. trans p2 (LIntChoice s b r) p4 /\
+        trans p3 alpha p4
+Proof
+  metis_tac[endpoint_local_confluence_int_choice]
+QED
+
+Theorem endpoint_local_confluence_receive:
+  ∀p1 s1 d1 r1 p2 p3 s2 d2 r2.
+  trans p1 (LReceive s1 d1 r1) p2 /\ trans p1 (LReceive s2 d2 r2) p3 /\ s1 <> s2
+  ==>
+  ?p4 p5. trans p2 (LReceive s2 d2 r2) p4 /\
+        trans p3 (LReceive s1 d1 r1) p5 /\
+        qcong p4 p5
+Proof
+  `∀p1 alpha p2 s1 d1 r1 p3 s2 d2 r2.
+  trans p1 alpha p2 /\ alpha = LReceive s1 d1 r1 /\
+  trans p1 (LReceive s2 d2 r2) p3 /\ s1 <> s2
+  ==>
+  ?p4 p5. trans p2 (LReceive s2 d2 r2) p4 /\
+        trans p3 (LReceive s1 d1 r1) p5 /\
+        qcong p4 p5` suffices_by metis_tac[] >>
+  Ho_Rewrite.PURE_REWRITE_TAC[GSYM AND_IMP_INTRO, GSYM PULL_FORALL]
+  >> ho_match_mp_tac trans_strongind
+  >> rpt strip_tac >> fs[] >> rveq
+  >- (* Enqueue *)
+     (qhdtm_x_assum `trans` (assume_tac o SIMP_RULE std_ss [Once trans_cases]) >>
+      fs[] >> rveq >> fs[] >> rveq >> fs[] >>
+      qmatch_goalsub_abbrev_tac `NEndpoint p2 s1 e` >>
+      dxrule trans_enqueue >> disch_then(qspecl_then [`s1`,`d2`,`e`] mp_tac) >>
+      unabbrev_all_tac >> strip_tac >>
+      asm_exists_tac >> simp[] >>
+      qmatch_goalsub_abbrev_tac `NEndpoint p2 s1 e` >>
+      qpat_x_assum `_ <> _` mp_tac >>
+      dxrule trans_enqueue >> disch_then(qspecl_then [`s1`,`d`,`e`] mp_tac) >>
+      unabbrev_all_tac >> rpt strip_tac >>
+      asm_exists_tac >> simp[] >>
+      simp[SNOC_APPEND] >> PURE_REWRITE_TAC[GSYM APPEND_ASSOC,APPEND] >>
+      match_mp_tac (qcong_queue_reorder'
+                    |> CONV_RULE(RESORT_FORALL_CONV rev)
+                    |> Q.SPEC `[]` |> REWRITE_RULE[APPEND_NIL]) >>
+      first_x_assum ACCEPT_TAC)
+  >- (* Par-L *)
+     (qhdtm_x_assum `trans` (assume_tac o SIMP_RULE std_ss [Once trans_cases]) >>
+      fs[] >> rveq >> fs[] >> rveq >> fs[] >>
+      metis_tac[trans_par_l,trans_par_r,qcong_refl,qcong_par]
+     )
+  >- (* Par-R *)
+     (qhdtm_x_assum `trans` (assume_tac o SIMP_RULE std_ss [Once trans_cases]) >>
+      fs[] >> rveq >> fs[] >> rveq >> fs[] >>
+      metis_tac[trans_par_l,trans_par_r,qcong_refl,qcong_par]
+     )
+QED
+
+Theorem endpoint_local_confluence_receive_choice:
+  ∀p1 s1 d r1 p2 p3 s2 b r2.
+  trans p1 (LReceive s1 d r1) p2 /\ trans p1 (LExtChoice s2 b r2) p3 /\ s1 <> s2
+  ==>
+  ?p4 p5. trans p2 (LExtChoice s2 b r2) p4 /\
+        trans p3 (LReceive s1 d r1) p5 /\
+        qcong p4 p5
+Proof
+  `∀p1 alpha p2 s1 d r1 p3 s2 b r2.
+  trans p1 alpha p2 /\ alpha = LReceive s1 d r1 /\
+  trans p1 (LExtChoice s2 b r2) p3 /\ s1 <> s2
+  ==>
+  ?p4 p5. trans p2 (LExtChoice s2 b r2) p4 /\
+        trans p3 (LReceive s1 d r1) p5 /\
+        qcong p4 p5` suffices_by metis_tac[] >>
+  Ho_Rewrite.PURE_REWRITE_TAC[GSYM AND_IMP_INTRO, GSYM PULL_FORALL]
+  >> ho_match_mp_tac trans_strongind
+  >> rpt strip_tac >> fs[] >> rveq
+  >- (* Enqueue *)
+     (qhdtm_x_assum `trans` (assume_tac o SIMP_RULE std_ss [Once trans_cases]) >>
+      fs[] >> rveq >> fs[] >> rveq >> fs[] >>
+      qmatch_goalsub_abbrev_tac `NEndpoint p2 s1 e` >>
+      TRY((rename1 `[0w]` >> dxrule trans_enqueue_choice_r) ORELSE dxrule trans_enqueue_choice_l >>
+          disch_then(qspecl_then [`s1`,`e`] mp_tac) >>
+          unabbrev_all_tac >> strip_tac >>
+          asm_exists_tac >> simp[] >>
+          qmatch_goalsub_abbrev_tac `NEndpoint p2 s1 e` >>
+          qpat_x_assum `_ <> _` mp_tac >>
+          dxrule trans_enqueue >> disch_then(qspecl_then [`s1`,`d`,`e`] mp_tac) >>
+          unabbrev_all_tac >> rpt strip_tac >>
+          asm_exists_tac >> simp[] >>
+          simp[SNOC_APPEND] >> PURE_REWRITE_TAC[GSYM APPEND_ASSOC,APPEND] >>
+          match_mp_tac (qcong_queue_reorder'
+                          |> CONV_RULE(RESORT_FORALL_CONV rev)
+                          |> Q.SPEC `[]` |> REWRITE_RULE[APPEND_NIL]) >>
+          first_x_assum ACCEPT_TAC)
+     )
+  >- (* Par-L *)
+     (qhdtm_x_assum `trans` (assume_tac o SIMP_RULE std_ss [Once trans_cases]) >>
+      fs[] >> rveq >> fs[] >> rveq >> fs[] >>
+      metis_tac[trans_par_l,trans_par_r,qcong_refl,qcong_par]
+     )
+  >- (* Par-R *)
+     (qhdtm_x_assum `trans` (assume_tac o SIMP_RULE std_ss [Once trans_cases]) >>
+      fs[] >> rveq >> fs[] >> rveq >> fs[] >>
+      metis_tac[trans_par_l,trans_par_r,qcong_refl,qcong_par]
+     )
+QED
+
+Theorem endpoint_local_confluence_choice:
+  ∀p1 s1 b1 r1 p2 p3 s2 b2 r2.
+  trans p1 (LExtChoice s1 b1 r1) p2 /\ trans p1 (LExtChoice s2 b2 r2) p3 /\ s1 <> s2
+  ==>
+  ?p4 p5. trans p2 (LExtChoice s2 b2 r2) p4 /\
+        trans p3 (LExtChoice s1 b1 r1) p5 /\
+        qcong p4 p5
+Proof
+  `∀p1 alpha p2 s1 b1 r1 p3 s2 b2 r2.
+  trans p1 alpha p2 /\ alpha = LExtChoice s1 b1 r1 /\
+  trans p1 (LExtChoice s2 b2 r2) p3 /\ s1 <> s2
+  ==>
+  ?p4 p5. trans p2 (LExtChoice s2 b2 r2) p4 /\
+        trans p3 (LExtChoice s1 b1 r1) p5 /\
+        qcong p4 p5` suffices_by metis_tac[] >>
+  Ho_Rewrite.PURE_REWRITE_TAC[GSYM AND_IMP_INTRO, GSYM PULL_FORALL]
+  >> ho_match_mp_tac trans_strongind
+  >> rpt strip_tac >> fs[] >> rveq
+  >- (* Enqueue-Choice-L *)
+     (qhdtm_x_assum `trans` (assume_tac o SIMP_RULE std_ss [Once trans_cases]) >>
+      fs[] >> rveq >> fs[] >> rveq >> fs[] >>
+      qmatch_goalsub_abbrev_tac `NEndpoint p2 s1 e` >>
+      TRY(
+       (rename1 `trans _ (_ _ F _) _ /\ trans _ _ _ /\ _` >> dxrule trans_enqueue_choice_r) ORELSE dxrule trans_enqueue_choice_l >>
+       disch_then(qspecl_then [`s1`,`e`] mp_tac) >>
+       unabbrev_all_tac >> strip_tac >>
+       asm_exists_tac >> simp[] >>
+       qmatch_goalsub_abbrev_tac `NEndpoint p2 s1 e` >>
+       qpat_x_assum `_ <> _` mp_tac >>
+       dxrule trans_enqueue_choice_l >> disch_then(qspecl_then [`s1`,`e`] mp_tac) >>
+       unabbrev_all_tac >> rpt strip_tac >>
+       asm_exists_tac >> simp[] >>
+       simp[SNOC_APPEND] >> PURE_REWRITE_TAC[GSYM APPEND_ASSOC,APPEND] >>
+       match_mp_tac (qcong_queue_reorder'
+                     |> CONV_RULE(RESORT_FORALL_CONV rev)
+                     |> Q.SPEC `[]` |> REWRITE_RULE[APPEND_NIL]) >>
+       first_x_assum ACCEPT_TAC))
+  >- (* Enqueue-Choice-R *)
+     (qhdtm_x_assum `trans` (assume_tac o SIMP_RULE std_ss [Once trans_cases]) >>
+      fs[] >> rveq >> fs[] >> rveq >> fs[] >>
+      qmatch_goalsub_abbrev_tac `NEndpoint p2 s1 e` >>
+      TRY(
+       (rename1 `trans _ (_ _ F _) _ /\ trans _ _ _ /\ _` >> dxrule trans_enqueue_choice_r) ORELSE dxrule trans_enqueue_choice_l >>
+       disch_then(qspecl_then [`s1`,`e`] mp_tac) >>
+       unabbrev_all_tac >> strip_tac >>
+       asm_exists_tac >> simp[] >>
+       qmatch_goalsub_abbrev_tac `NEndpoint p2 s1 e` >>
+       qpat_x_assum `_ <> _` mp_tac >>
+       dxrule trans_enqueue_choice_r >> disch_then(qspecl_then [`s1`,`e`] mp_tac) >>
+       unabbrev_all_tac >> rpt strip_tac >>
+       asm_exists_tac >> simp[] >>
+       simp[SNOC_APPEND] >> PURE_REWRITE_TAC[GSYM APPEND_ASSOC,APPEND] >>
+       match_mp_tac (qcong_queue_reorder'
+                     |> CONV_RULE(RESORT_FORALL_CONV rev)
+                     |> Q.SPEC `[]` |> REWRITE_RULE[APPEND_NIL]) >>
+       first_x_assum ACCEPT_TAC))
+  >- (* Par-L *)
+     (qhdtm_x_assum `trans` (assume_tac o SIMP_RULE std_ss [Once trans_cases]) >>
+      fs[] >> rveq >> fs[] >> rveq >> fs[] >>
+      metis_tac[trans_par_l,trans_par_r,qcong_refl,qcong_par]
+     )
+  >- (* Par-R *)
+     (qhdtm_x_assum `trans` (assume_tac o SIMP_RULE std_ss [Once trans_cases]) >>
+      fs[] >> rveq >> fs[] >> rveq >> fs[] >>
+      metis_tac[trans_par_l,trans_par_r,qcong_refl,qcong_par]
+     )
+QED
+
+Theorem endpoint_local_confluence_tau_receive:
+  ∀p1 p2 p3 s d r.
+  trans p1 LTau p2 /\ trans p1 (LReceive s d r) p3 /\ p2 <> p3 /\
+  ALL_DISTINCT (MAP FST (endpoints p1)) /\
+  ~MEM s (MAP FST (endpoints p1))
+  ==>
+  ?p4 p5. trans p2 (LReceive s d r) p4 /\
+        trans p3 LTau p5 /\
+        qcong p4 p5
+Proof
+  `∀p1 alpha p2 p3 s d r.
+  trans p1 alpha p2 /\ alpha = LTau /\ trans p1 (LReceive s d r) p3 /\ p2 <> p3 /\
+  ALL_DISTINCT (MAP FST (endpoints p1)) /\
+  ~MEM s (MAP FST (endpoints p1))
+  ==>
+  ?p4 p5. trans p2 (LReceive s d r) p4 /\
+        trans p3 LTau p5 /\
+        qcong p4 p5` suffices_by metis_tac[]
+  >> Ho_Rewrite.PURE_REWRITE_TAC[GSYM AND_IMP_INTRO, GSYM PULL_FORALL]
+  >> ho_match_mp_tac trans_strongind
+  >> rpt strip_tac >> fs[] >> rveq
+  >- (* Com-L *)
+     (qhdtm_x_assum `trans` (assume_tac o SIMP_RULE std_ss [Once trans_cases]) >>
+      fs[] >> rveq >> fs[] >> rveq >> fs[]
+      >- (fs[endpoints_def,ALL_DISTINCT_APPEND] >>
+          drule endpoint_local_confluence_send >> disch_then drule >>
+          impl_tac >-
+            (simp[] >> metis_tac[sender_is_endpoint,receiver_is_endpoint]) >>
+          strip_tac >>
+          metis_tac[trans_com_l,trans_par_l,qcong_refl,qcong_sym,qcong_par])
+      >- (fs[endpoints_def,ALL_DISTINCT_APPEND] >>
+          drule endpoint_local_confluence_send >> disch_then drule >>
+          impl_tac >-
+            (simp[] >>
+             metis_tac[trans_distinct_residual,label_rel_def,
+                       receive_ext_choice_rel_def,sender_is_endpoint,
+                       receiver_is_endpoint,label_distinct]) >>
+          strip_tac >>
+          metis_tac[trans_com_l,trans_par_l,qcong_refl,qcong_sym,qcong_par]
+         )
+      >- (fs[endpoints_def,ALL_DISTINCT_APPEND] >>
+          imp_res_tac receiver_is_endpoint >>
+          imp_res_tac sender_is_endpoint >>
+          dxrule endpoint_local_confluence_receive >>
+          disch_then dxrule >>
+          impl_tac >- metis_tac[] >>
+          strip_tac >>
+          metis_tac[trans_com_l,trans_par_r,qcong_refl,qcong_sym,qcong_par])
+      >- (fs[endpoints_def,ALL_DISTINCT_APPEND] >>
+          imp_res_tac receiver_is_endpoint >>
+          imp_res_tac sender_is_endpoint >>
+          dxrule endpoint_local_confluence_receive >>
+          disch_then dxrule >>
+          impl_tac >- metis_tac[] >>
+          strip_tac >>
+          metis_tac[trans_com_l,trans_par_r,qcong_refl,qcong_sym,qcong_par]))
+  >- (* Com-R *)
+     (qhdtm_x_assum `trans` (assume_tac o SIMP_RULE std_ss [Once trans_cases]) >>
+      fs[] >> rveq >> fs[] >> rveq >> fs[]
+      >- (fs[endpoints_def,ALL_DISTINCT_APPEND] >>
+          imp_res_tac receiver_is_endpoint >>
+          imp_res_tac sender_is_endpoint >>
+          dxrule endpoint_local_confluence_receive >>
+          disch_then dxrule >>
+          impl_tac >- metis_tac[] >>
+          strip_tac >>
+          metis_tac[trans_com_r,trans_par_l,qcong_refl,qcong_sym,qcong_par])
+      >- (fs[endpoints_def,ALL_DISTINCT_APPEND] >>
+          imp_res_tac receiver_is_endpoint >>
+          imp_res_tac sender_is_endpoint >>
+          dxrule endpoint_local_confluence_receive >>
+          disch_then dxrule >>
+          impl_tac >- metis_tac[] >>
+          strip_tac >>
+          metis_tac[trans_com_r,trans_par_l,qcong_refl,qcong_sym,qcong_par])
+      >- (fs[endpoints_def,ALL_DISTINCT_APPEND] >>
+          drule endpoint_local_confluence_send >> disch_then drule >>
+          impl_tac >-
+            (simp[] >>
+             metis_tac[sender_is_endpoint,receiver_is_endpoint,trans_distinct_residual,
+                       label_rel_def,receive_ext_choice_rel_def,label_distinct]) >>
+          strip_tac >>
+          metis_tac[trans_com_r,trans_par_r,qcong_refl,qcong_sym,qcong_par])
+      >- (fs[endpoints_def,ALL_DISTINCT_APPEND] >>
+          drule endpoint_local_confluence_send >> disch_then drule >>
+          impl_tac >-
+            (simp[] >>
+             metis_tac[sender_is_endpoint,receiver_is_endpoint,trans_distinct_residual,
+                       label_distinct]) >>
+          strip_tac >>
+          metis_tac[trans_com_r,trans_par_r,qcong_refl,qcong_sym,qcong_par]))
+  >- (* Com-Choice-L *)
+     (qhdtm_x_assum `trans` (assume_tac o SIMP_RULE std_ss [Once trans_cases]) >>
+      fs[] >> rveq >> fs[] >> rveq >> fs[]
+      >- (fs[endpoints_def,ALL_DISTINCT_APPEND] >>
+          drule endpoint_local_confluence_int_choice >> disch_then drule >>
+          impl_tac >-
+            (simp[] >> metis_tac[choice_sender_is_endpoint,choice_receiver_is_endpoint,receiver_is_endpoint]) >>
+          strip_tac >>
+          metis_tac[trans_com_choice_l,trans_par_l,qcong_refl,qcong_sym,qcong_par])
+      >- (fs[endpoints_def,ALL_DISTINCT_APPEND] >>
+          drule endpoint_local_confluence_int_choice >> disch_then drule >>
+          impl_tac >-
+            (simp[] >>
+             metis_tac[trans_distinct_residual,label_rel_def,
+                       receive_ext_choice_rel_def,choice_sender_is_endpoint,
+                       choice_receiver_is_endpoint,
+                       receiver_is_endpoint,label_distinct]) >>
+          strip_tac >>
+          metis_tac[trans_com_choice_l,trans_par_l,qcong_refl,qcong_sym,qcong_par]
+         )
+      >- (fs[endpoints_def,ALL_DISTINCT_APPEND] >>
+          imp_res_tac receiver_is_endpoint >>
+          imp_res_tac choice_sender_is_endpoint >>
+          imp_res_tac choice_receiver_is_endpoint >>
+          dxrule endpoint_local_confluence_receive_choice >>
+          disch_then dxrule >>
+          impl_tac >- metis_tac[] >>
+          strip_tac >>
+          metis_tac[trans_com_choice_l,trans_par_r,qcong_refl,qcong_sym,qcong_par])
+      >- (fs[endpoints_def,ALL_DISTINCT_APPEND] >>
+          imp_res_tac receiver_is_endpoint >>
+          imp_res_tac choice_sender_is_endpoint >>
+          imp_res_tac choice_receiver_is_endpoint >>
+          dxrule endpoint_local_confluence_receive_choice >>
+          disch_then dxrule >>
+          impl_tac >- metis_tac[] >>
+          strip_tac >>
+          metis_tac[trans_com_choice_l,trans_par_r,qcong_refl,qcong_sym,qcong_par]))
+  >- (* Com-R *)
+     (qhdtm_x_assum `trans` (assume_tac o SIMP_RULE std_ss [Once trans_cases]) >>
+      fs[] >> rveq >> fs[] >> rveq >> fs[]
+      >- (fs[endpoints_def,ALL_DISTINCT_APPEND] >>
+          imp_res_tac receiver_is_endpoint >>
+          imp_res_tac choice_sender_is_endpoint >>
+          imp_res_tac choice_receiver_is_endpoint >>
+          dxrule endpoint_local_confluence_receive_choice >>
+          disch_then dxrule >>
+          impl_tac >- metis_tac[choice_sender_is_endpoint] >>
+          strip_tac >>
+          metis_tac[trans_com_choice_r,trans_par_l,qcong_refl,qcong_sym,qcong_par])
+      >- (fs[endpoints_def,ALL_DISTINCT_APPEND] >>
+          imp_res_tac receiver_is_endpoint >>
+          imp_res_tac choice_sender_is_endpoint >>
+          imp_res_tac choice_sender_is_endpoint >>
+          dxrule endpoint_local_confluence_receive_choice >>
+          disch_then dxrule >>
+          impl_tac >- metis_tac[] >>
+          strip_tac >>
+          metis_tac[trans_com_choice_r,trans_par_l,qcong_refl,qcong_sym,qcong_par])
+      >- (fs[endpoints_def,ALL_DISTINCT_APPEND] >>
+          drule endpoint_local_confluence_int_choice >> disch_then drule >>
+          impl_tac >-
+            (simp[] >>
+             metis_tac[sender_is_endpoint,receiver_is_endpoint,trans_distinct_residual,
+                       choice_receiver_is_endpoint,choice_sender_is_endpoint,
+                       label_rel_def,receive_ext_choice_rel_def,label_distinct]) >>
+          strip_tac >>
+          metis_tac[trans_com_choice_r,trans_par_r,qcong_refl,qcong_sym,qcong_par])
+      >- (fs[endpoints_def,ALL_DISTINCT_APPEND] >>
+          drule endpoint_local_confluence_int_choice >> disch_then drule >>
+          impl_tac >-
+            (simp[] >>
+             metis_tac[sender_is_endpoint,receiver_is_endpoint,trans_distinct_residual,
+                       choice_sender_is_endpoint,choice_receiver_is_endpoint,
+                       label_distinct]) >>
+          strip_tac >>
+          metis_tac[trans_com_choice_r,trans_par_r,qcong_refl,qcong_sym,qcong_par]))
+  >- (* Dequeue *)
+     (qhdtm_x_assum `trans` (assume_tac o SIMP_RULE std_ss [Once trans_cases]) >>
+      fs[] >> rveq >> fs[] >> rveq >> fs[] >>
+      qmatch_goalsub_abbrev_tac `trans (NEndpoint p2 s1 e) (LReceive _ data _)` >>
+      dxrule trans_enqueue >>
+      disch_then(qspecl_then [`s1`,`data`,`e`] assume_tac) >>
+      asm_exists_tac >> simp[] >> unabbrev_all_tac >>
+      qmatch_goalsub_abbrev_tac `qcong a1` >>
+      qexists_tac `a1` >>
+      simp[qcong_refl] >>
+      qunabbrev_tac `a1` >>
+      simp[SNOC_APPEND] >>
+      PURE_ONCE_REWRITE_TAC[GSYM APPEND_ASSOC] >>
+      match_mp_tac(trans_dequeue'
+                   |> REWRITE_RULE[SNOC_APPEND,FLAT_APPEND,FLAT,APPEND_NIL]) >>
+      simp[])
+  >- (* ExtChoice-L *)
+     (qhdtm_x_assum `trans` (assume_tac o SIMP_RULE std_ss [Once trans_cases]) >>
+      fs[] >> rveq >> fs[] >> rveq >> fs[] >>
+      qmatch_goalsub_abbrev_tac `trans (NEndpoint p2 s1 e1) (LReceive _ data _)` >>
+      dxrule trans_enqueue >>
+      disch_then(qspecl_then [`s1`,`data`,`e1`] assume_tac) >>
+      asm_exists_tac >> simp[] >> unabbrev_all_tac >>
+      qmatch_goalsub_abbrev_tac `qcong a1` >>
+      qexists_tac `a1` >>
+      simp[qcong_refl] >>
+      qunabbrev_tac `a1` >>
+      simp[SNOC_APPEND] >>
+      PURE_ONCE_REWRITE_TAC[GSYM APPEND_ASSOC] >>
+      match_mp_tac(trans_ext_choice_l'
+                   |> REWRITE_RULE[SNOC_APPEND,FLAT_APPEND,FLAT,APPEND_NIL]) >>
+      simp[]
+     )
+  >- (* ExtChoice-R *)
+     (qhdtm_x_assum `trans` (assume_tac o SIMP_RULE std_ss [Once trans_cases]) >>
+      fs[] >> rveq >> fs[] >> rveq >> fs[] >>
+      qmatch_goalsub_abbrev_tac `trans (NEndpoint p2 s1 e2) (LReceive _ data _)` >>
+      dxrule trans_enqueue >>
+      disch_then(qspecl_then [`s1`,`data`,`e2`] assume_tac) >>
+      asm_exists_tac >> simp[] >> unabbrev_all_tac >>
+      qmatch_goalsub_abbrev_tac `qcong a1` >>
+      qexists_tac `a1` >>
+      simp[qcong_refl] >>
+      qunabbrev_tac `a1` >>
+      simp[SNOC_APPEND] >>
+      PURE_ONCE_REWRITE_TAC[GSYM APPEND_ASSOC] >>
+      match_mp_tac(trans_ext_choice_r'
+                   |> REWRITE_RULE[SNOC_APPEND,FLAT_APPEND,FLAT,APPEND_NIL]) >>
+      simp[]
+     )
+  >- (* If-L *)
+     (qhdtm_x_assum `trans` (assume_tac o SIMP_RULE std_ss [Once trans_cases]) >>
+      fs[] >> rveq >> fs[] >> rveq >> fs[] >>
+      qmatch_goalsub_abbrev_tac `trans (NEndpoint p2 s1 e1) (LReceive _ data _)` >>
+      dxrule trans_enqueue >>
+      disch_then(qspecl_then [`s1`,`data`,`e1`] assume_tac) >>
+      asm_exists_tac >> simp[] >> unabbrev_all_tac >>
+      qmatch_goalsub_abbrev_tac `qcong a1` >>
+      qexists_tac `a1` >>
+      simp[qcong_refl] >>
+      unabbrev_all_tac >>
+      match_mp_tac trans_if_true >>
+      simp[]
+     )
+  >- (* If-R *)
+     (qhdtm_x_assum `trans` (assume_tac o SIMP_RULE std_ss [Once trans_cases]) >>
+      fs[] >> rveq >> fs[] >> rveq >> fs[] >>
+      qmatch_goalsub_abbrev_tac `trans (NEndpoint p2 s1 ee) (LReceive _ data _)` >>
+      dxrule trans_enqueue >>
+      disch_then(qspecl_then [`s1`,`data`,`ee`] assume_tac) >>
+      asm_exists_tac >> simp[] >> unabbrev_all_tac >>
+      qmatch_goalsub_abbrev_tac `qcong a1` >>
+      qexists_tac `a1` >>
+      simp[qcong_refl] >>
+      unabbrev_all_tac >>
+      match_mp_tac trans_if_false >>
+      simp[]
+     )
+  >- (* Let *)
+     (qhdtm_x_assum `trans` (assume_tac o SIMP_RULE std_ss [Once trans_cases]) >>
+      fs[] >> rveq >> fs[] >> rveq >> fs[] >>
+      qmatch_goalsub_abbrev_tac `trans (NEndpoint p2 s1 ee) (LReceive _ data _)` >>
+      dxrule trans_enqueue >>
+      disch_then(qspecl_then [`s1`,`data`,`ee`] assume_tac) >>
+      asm_exists_tac >> simp[] >> unabbrev_all_tac >>
+      qmatch_goalsub_abbrev_tac `qcong a1` >>
+      qexists_tac `a1` >>
+      simp[qcong_refl] >>
+      unabbrev_all_tac >>
+      simp[] >>
+      match_mp_tac trans_let' >>
+      simp[]
+     )
+  >- (* Par-L *)
+     (qhdtm_x_assum `trans` (assume_tac o SIMP_RULE std_ss [Once trans_cases]) >>
+      fs[] >> rveq >> fs[] >> rveq >> fs[]
+      >- (fs[endpoints_def,ALL_DISTINCT_APPEND] >>
+          metis_tac[qcong_refl,qcong_par,trans_par_l])
+      >- (metis_tac[trans_par_l,trans_par_r,qcong_par,qcong_refl])
+      >- (metis_tac[trans_par_l,trans_par_r,qcong_par,qcong_refl]))
+  >- (* Par-R *)
+     (qhdtm_x_assum `trans` (assume_tac o SIMP_RULE std_ss [Once trans_cases]) >>
+      fs[] >> rveq >> fs[] >> rveq >> fs[]
+      >- metis_tac[trans_par_l,trans_par_r,qcong_par,qcong_refl] >>
+      fs[endpoints_def,ALL_DISTINCT_APPEND] >>
+      metis_tac[qcong_refl,qcong_par,trans_par_r,trans_par_l])
+QED
+
+Theorem endpoint_local_confluence_tau_choice:
+  ∀p1 p2 p3 s b r.
+  trans p1 LTau p2 /\ trans p1 (LExtChoice s b r) p3 /\ p2 <> p3 /\
+  ALL_DISTINCT (MAP FST (endpoints p1)) /\
+  ~MEM s (MAP FST (endpoints p1))
+  ==>
+  ?p4 p5. trans p2 (LExtChoice s b r) p4 /\
+        trans p3 LTau p5 /\
+        qcong p4 p5
+Proof
+ Cases_on `b` >>
+ metis_tac[endpoint_local_confluence_tau_receive,trans_ext_choice_T_receive,
+           trans_ext_choice_F_receive]
+QED
+
+Theorem endpoint_local_confluence_tau:
+  ∀p1 p2 p3.
+  trans p1 LTau p2 /\ trans p1 LTau p3 /\ p2 <> p3 /\
+  ALL_DISTINCT (MAP FST (endpoints p1))
+  ==>
+  ?p4 p5. trans p2 LTau p4 /\
+        trans p3 LTau p5 /\
+        qcong p4 p5
+Proof
+  `∀p1 alpha p2.
+    trans p1 alpha p2 ==> !p3. alpha = LTau /\ trans p1 LTau p3 /\ p2 <> p3 /\
+    ALL_DISTINCT (MAP FST (endpoints p1))
+    ==>
+    ?p4 p5. trans p2 LTau p4 /\
+            trans p3 LTau p5 /\
+            qcong p4 p5` suffices_by metis_tac[]
+  >> ho_match_mp_tac trans_strongind
+  >> rpt strip_tac >> fs[] >> rveq
+  >- (* Com-L *)
+     (qhdtm_x_assum `trans` (assume_tac o SIMP_RULE std_ss [Once trans_cases]) >>
+      fs[] >> rveq >> fs[] >> rveq >> fs[endpoints_def,ALL_DISTINCT_APPEND]
+      >- (qmatch_asmsub_abbrev_tac `trans _ (LSend s1 _ _)` >>
+          qpat_x_assum `trans _ (LSend _ _ _) _` mp_tac >>
+          qmatch_asmsub_abbrev_tac `trans _ (LSend s2 _ _)` >>
+          strip_tac >>
+          rpt(qhdtm_x_assum `Abbrev` kall_tac) >>
+          Cases_on `s1 = s2` >-
+            (rveq >>
+             fs[endpoints_def,ALL_DISTINCT_APPEND] >>
+             dxrule_all_then strip_assume_tac trans_same_sender_determ >>
+             rveq >> fs[]) >>
+          imp_res_tac sender_is_endpoint >>
+          imp_res_tac receiver_is_endpoint >>
+          dxrule endpoint_local_confluence_send >>
+          disch_then dxrule >>
+          impl_tac >- (simp[] >> metis_tac[]) >>
+          strip_tac >>
+          dxrule_all_then strip_assume_tac endpoint_local_confluence_receive >>
+          metis_tac[trans_com_l,qcong_par,qcong_sym,qcong_refl])
+      >- (qmatch_asmsub_abbrev_tac `trans _ (LSend s1 _ _)` >>
+          qpat_x_assum `trans _ (LSend _ _ _) _` mp_tac >>
+          qmatch_asmsub_abbrev_tac `trans _ (LSend s2 _ _)` >>         
+          strip_tac >>
+          rpt(qhdtm_x_assum `Abbrev` kall_tac) >>
+          Cases_on `s1 = s2` >-
+            (rveq >>
+             fs[endpoints_def,ALL_DISTINCT_APPEND] >>
+             dxrule_all_then strip_assume_tac trans_same_sender_determ >>
+             rveq >> fs[] >> metis_tac[trans_same_receiver_determ]) >>
+          imp_res_tac sender_is_endpoint >>
+          imp_res_tac receiver_is_endpoint >>
+          drule_then assume_tac (GEN_ALL trans_different_sender) >>
+          qpat_x_assum `trans _ (LSend _ _ _) _` mp_tac >>
+          first_x_assum drule >> impl_tac >- simp[] >>
+          rpt strip_tac >>
+          dxrule endpoint_local_confluence_send >>
+          disch_then dxrule >>
+          impl_tac >- (simp[] >> metis_tac[]) >>
+          strip_tac >>
+          dxrule_all_then strip_assume_tac endpoint_local_confluence_receive >>
+          metis_tac[trans_com_l,qcong_par,qcong_sym,qcong_refl])
+      >- (imp_res_tac sender_is_endpoint >>
+          imp_res_tac receiver_is_endpoint >>
+          drule(GEN_ALL trans_send_receive_distinct) >>
+          disch_then drule >>
+          strip_tac >>
+          qpat_x_assum `trans _ (LSend _ _ _) _` mp_tac >>
+          dxrule_then assume_tac endpoint_local_confluence_send >>
+          strip_tac >> first_x_assum dxrule >>
+          impl_tac >- (simp[] >> metis_tac[]) >>
+          qpat_x_assum `trans _ (LSend _ _ _) _` mp_tac >>
+          dxrule_then assume_tac endpoint_local_confluence_send >>
+          strip_tac >> first_x_assum dxrule >>
+          impl_tac >- simp[] >>
+          rpt strip_tac >>
+          metis_tac[trans_com_l,trans_com_r,qcong_par,qcong_sym,qcong_refl])
+      >- (imp_res_tac sender_is_endpoint >>
+          imp_res_tac receiver_is_endpoint >>
+          qpat_x_assum `trans _ (LSend _ _ _) _` mp_tac >>
+          drule(GEN_ALL trans_send_receive_distinct) >>
+          disch_then drule >>
+          strip_tac >>
+          dxrule_then assume_tac endpoint_local_confluence_send >>
+          strip_tac >> first_x_assum dxrule >>
+          impl_tac >- (simp[] >> metis_tac[]) >>
+          qpat_x_assum `trans _ (LSend _ _ _) _` mp_tac >>
+          dxrule_then assume_tac endpoint_local_confluence_send >>
+          strip_tac >> first_x_assum dxrule >>
+          impl_tac >- simp[] >>
+          rpt strip_tac >>
+          metis_tac[trans_com_l,trans_com_r,qcong_par,qcong_sym,qcong_refl])
+      >- (fs[endpoints_def,ALL_DISTINCT_APPEND] >>
+          drule(GEN_ALL trans_send_choice_distinct_senders) >>
+          rpt(disch_then drule) >> strip_tac >>
+          imp_res_tac sender_is_endpoint >>
+          imp_res_tac receiver_is_endpoint >>
+          imp_res_tac choice_sender_is_endpoint >>
+          imp_res_tac choice_receiver_is_endpoint >>
+          dxrule_all endpoint_local_confluence_receive_choice >>
+          dxrule endpoint_local_confluence_send >>
+          disch_then dxrule >>
+          impl_tac >- (simp[] >> metis_tac[]) >>
+          metis_tac[trans_com_l,trans_com_choice_l,qcong_par,qcong_sym,qcong_refl])
+      >- (fs[endpoints_def,ALL_DISTINCT_APPEND] >>
+          drule(GEN_ALL trans_send_choice_distinct_senders) >>
+          rpt(disch_then drule) >> strip_tac >>
+          imp_res_tac sender_is_endpoint >>
+          imp_res_tac receiver_is_endpoint >>
+          imp_res_tac choice_sender_is_endpoint >>
+          imp_res_tac choice_receiver_is_endpoint >>
+          dxrule_all endpoint_local_confluence_receive_choice >>
+          drule(GEN_ALL trans_send_choice_distinct_senders) >>
+          rpt(disch_then drule) >> strip_tac >>
+          drule endpoint_local_confluence_send >>
+          disch_then drule >>
+          impl_tac >- (simp[] >>
+                       conj_tac >-
+                        (match_mp_tac trans_distinct_residual >>
+                         asm_exists_tac >> rw[] >> asm_exists_tac >>
+                         rw[label_rel_def,receive_ext_choice_rel_def]) >>
+                       metis_tac[]) >>
+          metis_tac[trans_com_l,trans_com_choice_l,qcong_par,qcong_sym,qcong_refl])      
+      >- (imp_res_tac sender_is_endpoint >>
+          imp_res_tac receiver_is_endpoint >>
+          imp_res_tac choice_sender_is_endpoint >>
+          imp_res_tac choice_receiver_is_endpoint >>
+          drule_then assume_tac trans_distinct_residual >>
+          qhdtm_x_assum `trans` mp_tac >>
+          pop_assum drule >>
+          impl_tac >- simp[label_rel_def,receive_ext_choice_rel_def] >>
+          strip_tac >>
+          drule_then assume_tac trans_distinct_residual >>
+          qhdtm_x_assum `trans` mp_tac >>
+          pop_assum drule >>
+          impl_tac >- simp[label_rel_def,receive_ext_choice_rel_def] >>
+          rpt strip_tac >>
+          dxrule(GEN_ALL endpoint_local_confluence_send_rotated) >>
+          disch_then dxrule >> impl_tac >- metis_tac[] >>
+          dxrule(GEN_ALL endpoint_local_confluence_int_choice_rotated) >>
+          disch_then drule >> impl_tac >- simp[] >>
+          metis_tac[trans_com_l,trans_com_choice_r,qcong_par,qcong_sym,qcong_refl])
+      >- (imp_res_tac sender_is_endpoint >>
+          imp_res_tac receiver_is_endpoint >>
+          imp_res_tac choice_sender_is_endpoint >>
+          imp_res_tac choice_receiver_is_endpoint >>
+          drule_then assume_tac trans_distinct_residual >>
+          qhdtm_x_assum `trans` mp_tac >>
+          pop_assum drule >>
+          impl_tac >- simp[label_rel_def,receive_ext_choice_rel_def] >>
+          strip_tac >>
+          drule_then assume_tac trans_distinct_residual >>
+          qhdtm_x_assum `trans` mp_tac >>
+          pop_assum drule >>
+          impl_tac >- simp[label_rel_def,receive_ext_choice_rel_def] >>
+          rpt strip_tac >>
+          dxrule(GEN_ALL endpoint_local_confluence_send_rotated) >>
+          disch_then dxrule >> impl_tac >- metis_tac[] >>
+          dxrule(GEN_ALL endpoint_local_confluence_int_choice_rotated) >>
+          disch_then drule >> impl_tac >- simp[] >>
+          metis_tac[trans_com_l,trans_com_choice_r,qcong_par,qcong_sym,qcong_refl])
+      >- (imp_res_tac sender_is_endpoint >>
+          imp_res_tac receiver_is_endpoint >>
+          dxrule endpoint_local_confluence_send >>
+          disch_then dxrule >>
+          impl_tac >- (simp[] >> metis_tac[]) >>
+          strip_tac >>
+          metis_tac[trans_com_l,trans_par_l,qcong_par,qcong_refl,qcong_sym])
+      >- (imp_res_tac sender_is_endpoint >>
+          imp_res_tac receiver_is_endpoint >>
+          drule_then assume_tac trans_distinct_residual >>
+          qhdtm_x_assum `trans` mp_tac >>
+          pop_assum drule >> impl_tac >- simp[label_rel_def,receive_ext_choice_rel_def] >>
+          rpt strip_tac >>
+          dxrule endpoint_local_confluence_send >>
+          disch_then dxrule >>
+          impl_tac >- (simp[] >> metis_tac[]) >>
+          strip_tac >>
+          metis_tac[trans_com_l,trans_par_l,qcong_par,qcong_refl,qcong_sym])
+      >- (imp_res_tac sender_is_endpoint >>
+          imp_res_tac receiver_is_endpoint >>
+          drule_then assume_tac trans_distinct_residual >>
+          qhdtm_x_assum `trans` mp_tac >>
+          pop_assum drule >> impl_tac >- simp[label_rel_def,receive_ext_choice_rel_def] >>
+          rpt strip_tac >>
+          dxrule endpoint_local_confluence_tau_receive >>
+          disch_then dxrule >>
+          impl_tac >- (simp[] >> metis_tac[]) >>
+          strip_tac >>
+          metis_tac[trans_com_l,trans_par_r,qcong_par,qcong_refl,qcong_sym])
+      >- (imp_res_tac sender_is_endpoint >>
+          imp_res_tac receiver_is_endpoint >>
+          drule_then assume_tac trans_distinct_residual >>
+          qhdtm_x_assum `trans` mp_tac >>
+          pop_assum drule >> impl_tac >- simp[label_rel_def,receive_ext_choice_rel_def] >>
+          rpt strip_tac >>
+          dxrule endpoint_local_confluence_tau_receive >>
+          disch_then dxrule >>
+          impl_tac >- (simp[] >> metis_tac[]) >>
+          strip_tac >>
+          metis_tac[trans_com_l,trans_par_r,qcong_par,qcong_refl,qcong_sym]))
+  >- (* Com-R *)
+     (qhdtm_x_assum `trans` (assume_tac o SIMP_RULE std_ss [Once trans_cases]) >>
+      fs[] >> rveq >> fs[] >> rveq >> fs[endpoints_def,ALL_DISTINCT_APPEND]
+      >- (imp_res_tac sender_is_endpoint >>
+          imp_res_tac receiver_is_endpoint >>
+          qpat_x_assum `trans _ (LSend _ _ _) _` mp_tac >>
+          drule(GEN_ALL trans_send_receive_distinct) >>
+          disch_then drule >>
+          strip_tac >>
+          dxrule_then assume_tac endpoint_local_confluence_send >>
+          strip_tac >> first_x_assum dxrule >>
+          impl_tac >- (simp[] >> metis_tac[]) >>
+          qpat_x_assum `trans _ (LSend _ _ _) _` mp_tac >>
+          dxrule_then assume_tac endpoint_local_confluence_send >>
+          strip_tac >> first_x_assum dxrule >>
+          impl_tac >- (simp[] >> metis_tac[]) >>
+          rpt strip_tac >>
+          metis_tac[trans_com_l,trans_com_r,qcong_par,qcong_sym,qcong_refl])
+      >- (imp_res_tac sender_is_endpoint >>
+          imp_res_tac receiver_is_endpoint >>
+          drule(GEN_ALL trans_send_receive_distinct) >>
+          disch_then drule >>
+          strip_tac >>
+          qpat_x_assum `trans _ (LSend _ _ _) _` mp_tac >>
+          dxrule_then assume_tac endpoint_local_confluence_send >>
+          strip_tac >> first_x_assum dxrule >>
+          impl_tac >- (simp[] >> metis_tac[]) >>
+          qpat_x_assum `trans _ (LSend _ _ _) _` mp_tac >>
+          dxrule_then assume_tac endpoint_local_confluence_send >>
+          strip_tac >> first_x_assum dxrule >>
+          impl_tac >- (simp[] >> metis_tac[]) >>
+          rpt strip_tac >>
+          metis_tac[trans_com_l,trans_com_r,qcong_par,qcong_sym,qcong_refl])      
+      >- (qmatch_asmsub_abbrev_tac `trans _ (LSend s1 _ _)` >>
+          qpat_x_assum `trans _ (LSend _ _ _) _` mp_tac >>
+          qmatch_asmsub_abbrev_tac `trans _ (LSend s2 _ _)` >>
+          strip_tac >>
+          rpt(qhdtm_x_assum `Abbrev` kall_tac) >>
+          Cases_on `s1 = s2` >-
+            (rveq >>
+             fs[endpoints_def,ALL_DISTINCT_APPEND] >>
+             dxrule(GEN_ALL trans_same_sender_determ) >>
+             disch_then dxrule >> impl_tac >- fs[] >>
+             strip_tac >>
+             rveq >> fs[] >> metis_tac[trans_same_receiver_determ]) >>
+          imp_res_tac sender_is_endpoint >>
+          imp_res_tac receiver_is_endpoint >>
+          drule_then assume_tac (GEN_ALL trans_different_sender) >>
+          qhdtm_x_assum `trans` mp_tac >>
+          pop_assum drule >> impl_tac >- simp[] >>
+          rpt strip_tac >>
+          dxrule endpoint_local_confluence_send >>
+          disch_then dxrule >>
+          impl_tac >- (simp[] >> metis_tac[]) >>
+          strip_tac >>
+          dxrule_all_then strip_assume_tac endpoint_local_confluence_receive >>
+          metis_tac[trans_com_r,qcong_par,qcong_sym,qcong_refl])
+      >- (qmatch_asmsub_abbrev_tac `trans _ (LSend s1 _ _)` >>
+          qpat_x_assum `trans _ (LSend _ _ _) _` mp_tac >>
+          qmatch_asmsub_abbrev_tac `trans _ (LSend s2 _ _)` >>
+          strip_tac >>
+          rpt(qhdtm_x_assum `Abbrev` kall_tac) >>
+          Cases_on `s1 = s2` >-
+            (rveq >>
+             fs[endpoints_def,ALL_DISTINCT_APPEND] >>
+             dxrule(GEN_ALL trans_same_sender_determ) >>
+             disch_then dxrule >> impl_tac >- fs[] >>
+             strip_tac >>
+             rveq >> fs[] >> metis_tac[trans_same_receiver_determ]) >>
+          imp_res_tac sender_is_endpoint >>
+          imp_res_tac receiver_is_endpoint >>
+          drule_then assume_tac (GEN_ALL trans_different_sender) >>
+          qhdtm_x_assum `trans` mp_tac >>
+          pop_assum drule >> impl_tac >- simp[] >>
+          rpt strip_tac >>
+          dxrule endpoint_local_confluence_send >>
+          disch_then dxrule >>
+          impl_tac >- (simp[] >> metis_tac[]) >>
+          strip_tac >>
+          dxrule_all_then strip_assume_tac endpoint_local_confluence_receive >>
+          metis_tac[trans_com_r,qcong_par,qcong_sym,qcong_refl])
+      >- (imp_res_tac sender_is_endpoint >>
+          imp_res_tac receiver_is_endpoint >>
+          imp_res_tac choice_sender_is_endpoint >>
+          imp_res_tac choice_receiver_is_endpoint >>
+          drule_then assume_tac trans_distinct_residual >>
+          qhdtm_x_assum `trans` mp_tac >>
+          pop_assum drule >>
+          impl_tac >- simp[label_rel_def,receive_ext_choice_rel_def] >>
+          strip_tac >>
+          drule_then assume_tac trans_distinct_residual >>
+          qhdtm_x_assum `trans` mp_tac >>
+          pop_assum drule >>
+          impl_tac >- simp[label_rel_def,receive_ext_choice_rel_def] >>
+          rpt strip_tac >>
+          dxrule(GEN_ALL endpoint_local_confluence_send_rotated) >>
+          disch_then dxrule >> impl_tac >- metis_tac[] >>
+          dxrule(GEN_ALL endpoint_local_confluence_int_choice_rotated) >>
+          disch_then drule >> impl_tac >- (simp[] >> metis_tac[]) >>
+          metis_tac[trans_com_r,trans_com_choice_l,qcong_par,qcong_sym,qcong_refl])
+      >- (imp_res_tac sender_is_endpoint >>
+          imp_res_tac receiver_is_endpoint >>
+          imp_res_tac choice_sender_is_endpoint >>
+          imp_res_tac choice_receiver_is_endpoint >>
+          drule_then assume_tac trans_distinct_residual >>
+          qhdtm_x_assum `trans` mp_tac >>
+          pop_assum drule >>
+          impl_tac >- simp[label_rel_def,receive_ext_choice_rel_def] >>
+          strip_tac >>
+          drule_then assume_tac trans_distinct_residual >>
+          qhdtm_x_assum `trans` mp_tac >>
+          pop_assum drule >>
+          impl_tac >- simp[label_rel_def,receive_ext_choice_rel_def] >>
+          rpt strip_tac >>
+          dxrule(GEN_ALL endpoint_local_confluence_send_rotated) >>
+          disch_then dxrule >> impl_tac >- metis_tac[] >>
+          dxrule(GEN_ALL endpoint_local_confluence_int_choice_rotated) >>
+          disch_then drule >> impl_tac >- (simp[] >> metis_tac[]) >>
+          metis_tac[trans_com_r,trans_com_choice_l,qcong_par,qcong_sym,qcong_refl])
+      >- (fs[endpoints_def,ALL_DISTINCT_APPEND] >>
+          drule(GEN_ALL trans_send_choice_distinct_senders) >>
+          rpt(disch_then drule) >> strip_tac >>
+          imp_res_tac sender_is_endpoint >>
+          imp_res_tac receiver_is_endpoint >>
+          imp_res_tac choice_sender_is_endpoint >>
+          imp_res_tac choice_receiver_is_endpoint >>
+          dxrule_all endpoint_local_confluence_receive_choice >>
+          drule(GEN_ALL trans_send_choice_distinct_senders) >>
+          rpt(disch_then drule) >> strip_tac >>
+          drule endpoint_local_confluence_send >>
+          disch_then drule >>
+          impl_tac >- (simp[] >>
+                       match_mp_tac trans_distinct_residual >>
+                       asm_exists_tac >> rw[] >> asm_exists_tac >>
+                       rw[label_rel_def,receive_ext_choice_rel_def]) >>
+          metis_tac[trans_com_r,trans_com_choice_r,qcong_par,qcong_sym,qcong_refl])
+      >- (fs[endpoints_def,ALL_DISTINCT_APPEND] >>
+          drule(GEN_ALL trans_send_choice_distinct_senders) >>
+          rpt(disch_then drule) >> strip_tac >>
+          imp_res_tac sender_is_endpoint >>
+          imp_res_tac receiver_is_endpoint >>
+          imp_res_tac choice_sender_is_endpoint >>
+          imp_res_tac choice_receiver_is_endpoint >>
+          dxrule_all endpoint_local_confluence_receive_choice >>
+          dxrule endpoint_local_confluence_send_rotated >>
+          disch_then dxrule >>
+          impl_tac >- (simp[] >> metis_tac[]) >>
+          metis_tac[trans_com_r,trans_com_choice_r,qcong_par,qcong_sym,qcong_refl])
+      >- (imp_res_tac sender_is_endpoint >>
+          imp_res_tac receiver_is_endpoint >>
+          drule_then assume_tac trans_distinct_residual >>
+          qhdtm_x_assum `trans` mp_tac >>
+          pop_assum drule >> impl_tac >- simp[label_rel_def,receive_ext_choice_rel_def] >>
+          rpt strip_tac >>
+          dxrule endpoint_local_confluence_tau_receive >>
+          disch_then dxrule >>
+          impl_tac >- (simp[] >> metis_tac[]) >>
+          strip_tac >>
+          metis_tac[trans_com_r,trans_par_l,qcong_par,qcong_refl,qcong_sym])
+      >- (imp_res_tac sender_is_endpoint >>
+          imp_res_tac receiver_is_endpoint >>
+          drule_then assume_tac trans_distinct_residual >>
+          qhdtm_x_assum `trans` mp_tac >>
+          pop_assum drule >> impl_tac >- simp[label_rel_def,receive_ext_choice_rel_def] >>
+          rpt strip_tac >>
+          dxrule endpoint_local_confluence_tau_receive >>
+          disch_then dxrule >>
+          impl_tac >- (simp[] >> metis_tac[]) >>
+          strip_tac >>
+          metis_tac[trans_com_r,trans_par_l,qcong_par,qcong_refl,qcong_sym])
+      >- (imp_res_tac sender_is_endpoint >>
+          imp_res_tac receiver_is_endpoint >>
+          drule_then assume_tac trans_distinct_residual >>
+          qhdtm_x_assum `trans` mp_tac >>
+          pop_assum drule >> impl_tac >- simp[label_rel_def,receive_ext_choice_rel_def] >>
+          rpt strip_tac >>
+          dxrule endpoint_local_confluence_send >>
+          disch_then dxrule >>
+          impl_tac >- (simp[] >> metis_tac[]) >>
+          strip_tac >>
+          metis_tac[trans_com_r,trans_par_r,qcong_par,qcong_refl,qcong_sym])
+      >- (imp_res_tac sender_is_endpoint >>
+          imp_res_tac receiver_is_endpoint >>
+          dxrule endpoint_local_confluence_send >>
+          disch_then dxrule >>
+          impl_tac >- (simp[] >> metis_tac[]) >>
+          strip_tac >>
+          metis_tac[trans_com_r,trans_par_r,qcong_par,qcong_refl,qcong_sym]))
+  >- (* Com-Choice-L *)
+     cheat
+  >- (* Com-Choice-R *)
+     cheat
+  >- (* Dequeue *)
+     (qhdtm_x_assum `trans` (assume_tac o SIMP_RULE std_ss [Once trans_cases]) >>
+      fs[] >> rveq >> fs[] >> rveq >> fs[] >>
+      fs[APPEND_EQ_APPEND_MID] >> rveq >>
+      fs[APPEND_EQ_SING |> CONV_RULE(LHS_CONV SYM_CONV)] >>
+      rveq >> fs[])
+  >- (* ExtChoice-L *)
+     (qhdtm_x_assum `trans` (assume_tac o SIMP_RULE std_ss [Once trans_cases]) >>
+      fs[] >> rveq >> fs[] >> rveq >> fs[] >>
+      fs[APPEND_EQ_APPEND_MID] >> rveq >>
+      fs[APPEND_EQ_SING |> CONV_RULE(LHS_CONV SYM_CONV)] >>
+      rveq >> fs[])
+  >- (* ExtChoice-R *)
+     (qhdtm_x_assum `trans` (assume_tac o SIMP_RULE std_ss [Once trans_cases]) >>
+      fs[] >> rveq >> fs[] >> rveq >> fs[] >>
+      fs[APPEND_EQ_APPEND_MID] >> rveq >>
+      fs[APPEND_EQ_SING |> CONV_RULE(LHS_CONV SYM_CONV)] >>
+      rveq >> fs[])
+  >- (* If-L *)
+     (qhdtm_x_assum `trans` (assume_tac o SIMP_RULE std_ss [Once trans_cases]) >>
+      fs[] >> rveq >> fs[])
+  >- (* If-R *)
+     (qhdtm_x_assum `trans` (assume_tac o SIMP_RULE std_ss [Once trans_cases]) >>
+      fs[] >> rveq >> fs[])
+  >- (* Let *)
+     (qhdtm_x_assum `trans` (assume_tac o SIMP_RULE std_ss [Once trans_cases]) >>
+      fs[] >> rveq >> fs[])
+  >- (* Par-L *)
+     (qhdtm_x_assum `trans` (assume_tac o SIMP_RULE std_ss [Once trans_cases]) >>
+      fs[] >> rveq >> fs[] >> rveq >> fs[]
+      >- (fs[endpoints_def,ALL_DISTINCT_APPEND] >>
+          qpat_x_assum `_ _ LTau _` assume_tac >>
+          drule endpoint_local_confluence_send >>
+          disch_then drule >>
+          impl_tac >- metis_tac[receiver_is_endpoint] >>
+          strip_tac >>
+          metis_tac[trans_com_l,trans_par_l,qcong_par,qcong_refl])
+      >- (fs[endpoints_def,ALL_DISTINCT_APPEND] >>
+          qpat_x_assum `_ _ LTau _` assume_tac >>
+          drule endpoint_local_confluence_send >>
+          disch_then drule >>
+          impl_tac >- (simp[] >> metis_tac[trans_distinct_residual,label_distinct,
+                                           label_rel_def,receive_ext_choice_rel_def,
+                                           sender_is_endpoint,receiver_is_endpoint]) >>
+          strip_tac >>
+          metis_tac[trans_com_l,trans_par_l,qcong_par,qcong_refl])
+      >- (fs[endpoints_def,ALL_DISTINCT_APPEND] >>
+          imp_res_tac sender_is_endpoint >>
+          imp_res_tac receiver_is_endpoint >>
+          drule endpoint_local_confluence_tau_receive >>
+          disch_then drule >>
+          impl_tac >- (simp[] >> metis_tac[]) >>
+          strip_tac >>
+          metis_tac[trans_com_r,trans_par_l,qcong_par,qcong_refl])
+      >- (fs[endpoints_def,ALL_DISTINCT_APPEND] >>
+          imp_res_tac sender_is_endpoint >>
+          imp_res_tac receiver_is_endpoint >>
+          drule endpoint_local_confluence_tau_receive >>
+          disch_then drule >>
+          impl_tac >- (simp[] >> metis_tac[trans_distinct_residual,label_distinct,
+                                           label_rel_def,receive_ext_choice_rel_def]) >>
+          strip_tac >>
+          metis_tac[trans_com_r,trans_par_l,qcong_par,qcong_refl])
+      >- (fs[endpoints_def,ALL_DISTINCT_APPEND] >>
+          qpat_x_assum `_ _ LTau _` assume_tac >>
+          drule endpoint_local_confluence_int_choice >>
+          disch_then drule >>
+          impl_tac >- metis_tac[choice_receiver_is_endpoint] >>
+          strip_tac >>
+          metis_tac[trans_com_choice_l,trans_par_l,qcong_par,qcong_refl])
+      >- (fs[endpoints_def,ALL_DISTINCT_APPEND] >>
+          qpat_x_assum `_ _ LTau _` assume_tac >>
+          drule endpoint_local_confluence_int_choice >>
+          disch_then drule >>
+          impl_tac >- (simp[] >> metis_tac[trans_distinct_residual,label_distinct,
+                                           label_rel_def,receive_ext_choice_rel_def,
+                                           choice_sender_is_endpoint,choice_receiver_is_endpoint]) >>
+          strip_tac >>
+          metis_tac[trans_com_choice_l,trans_par_l,qcong_par,qcong_refl])
+      >- (fs[endpoints_def,ALL_DISTINCT_APPEND] >>
+          imp_res_tac choice_sender_is_endpoint >>
+          imp_res_tac choice_receiver_is_endpoint >>
+          drule endpoint_local_confluence_tau_choice >>
+          disch_then drule >>
+          impl_tac >- (simp[] >> metis_tac[]) >>
+          strip_tac >>
+          metis_tac[trans_com_choice_r,trans_par_l,qcong_par,qcong_refl])
+      >- (fs[endpoints_def,ALL_DISTINCT_APPEND] >>
+          imp_res_tac choice_sender_is_endpoint >>
+          imp_res_tac choice_receiver_is_endpoint >>
+          drule endpoint_local_confluence_tau_choice >>
+          disch_then drule >>
+          impl_tac >- (simp[] >> metis_tac[trans_distinct_residual,label_distinct,
+                                           label_rel_def,receive_ext_choice_rel_def]) >>
+          strip_tac >>
+          metis_tac[trans_com_choice_r,trans_par_l,qcong_par,qcong_refl])
+      >- (fs[endpoints_def,ALL_DISTINCT_APPEND] >>
+          metis_tac[trans_par_l,qcong_par,qcong_refl])
+      >- (fs[endpoints_def,ALL_DISTINCT_APPEND] >>
+          metis_tac[trans_par_r,trans_par_l,qcong_par,qcong_refl])
+      >- (fs[endpoints_def,ALL_DISTINCT_APPEND] >>
+          metis_tac[trans_par_r,trans_par_l,qcong_par,qcong_refl]))
+  >- (* Par-R *)
+     (qhdtm_x_assum `trans` (assume_tac o SIMP_RULE std_ss [Once trans_cases]) >>
+      fs[] >> rveq >> fs[] >> rveq >> fs[]
+      >- (fs[endpoints_def,ALL_DISTINCT_APPEND] >>
+          imp_res_tac sender_is_endpoint >>
+          imp_res_tac receiver_is_endpoint >>
+          drule endpoint_local_confluence_tau_receive >>
+          disch_then drule >>
+          impl_tac >- (simp[] >> metis_tac[trans_distinct_residual,label_distinct,
+                                           label_rel_def,receive_ext_choice_rel_def]) >>
+          strip_tac >>
+          metis_tac[trans_com_l,trans_par_r,qcong_par,qcong_refl])
+      >- (fs[endpoints_def,ALL_DISTINCT_APPEND] >>
+          imp_res_tac sender_is_endpoint >>
+          imp_res_tac receiver_is_endpoint >>
+          drule endpoint_local_confluence_tau_receive >>
+          disch_then drule >>
+          impl_tac >- (simp[] >> metis_tac[trans_distinct_residual,label_distinct,
+                                           label_rel_def,receive_ext_choice_rel_def]) >>
+          strip_tac >>
+          metis_tac[trans_com_l,trans_par_r,qcong_par,qcong_refl])
+      >- (fs[endpoints_def,ALL_DISTINCT_APPEND] >>
+          qpat_x_assum `_ _ LTau _` assume_tac >>
+          drule endpoint_local_confluence_send >>
+          disch_then drule >>
+          impl_tac >- (simp[] >> metis_tac[trans_distinct_residual,label_distinct,
+                                           label_rel_def,receive_ext_choice_rel_def,
+                                           sender_is_endpoint,receiver_is_endpoint]) >>
+          strip_tac >>
+          metis_tac[trans_com_r,trans_par_r,qcong_par,qcong_refl])
+      >- (fs[endpoints_def,ALL_DISTINCT_APPEND] >>
+          qpat_x_assum `_ _ LTau _` assume_tac >>
+          drule endpoint_local_confluence_send >>
+          disch_then drule >>
+          impl_tac >- (simp[] >> metis_tac[trans_distinct_residual,label_distinct,
+                                           label_rel_def,receive_ext_choice_rel_def,
+                                           sender_is_endpoint,receiver_is_endpoint]) >>
+          strip_tac >>
+          metis_tac[trans_com_r,trans_par_r,qcong_par,qcong_refl])
+      >- (fs[endpoints_def,ALL_DISTINCT_APPEND] >>
+          imp_res_tac choice_sender_is_endpoint >>
+          imp_res_tac choice_receiver_is_endpoint >>
+          drule endpoint_local_confluence_tau_choice >>
+          disch_then drule >>
+          impl_tac >- (simp[] >> metis_tac[trans_distinct_residual,label_distinct,
+                                           label_rel_def,receive_ext_choice_rel_def]) >>
+          strip_tac >>
+          metis_tac[trans_com_choice_l,trans_par_r,qcong_par,qcong_refl])
+      >- (fs[endpoints_def,ALL_DISTINCT_APPEND] >>
+          imp_res_tac choice_sender_is_endpoint >>
+          imp_res_tac choice_receiver_is_endpoint >>
+          drule endpoint_local_confluence_tau_choice >>
+          disch_then drule >>
+          impl_tac >- (simp[] >> metis_tac[trans_distinct_residual,label_distinct,
+                                           label_rel_def,receive_ext_choice_rel_def]) >>
+          strip_tac >>
+          metis_tac[trans_com_choice_l,trans_par_r,qcong_par,qcong_refl])
+      >- (fs[endpoints_def,ALL_DISTINCT_APPEND] >>
+          qpat_x_assum `_ _ LTau _` assume_tac >>
+          drule endpoint_local_confluence_int_choice >>
+          disch_then drule >>
+          impl_tac >- (simp[] >> metis_tac[trans_distinct_residual,label_distinct,
+                                           label_rel_def,receive_ext_choice_rel_def,
+                                           choice_sender_is_endpoint,choice_receiver_is_endpoint]) >>
+          strip_tac >>
+          metis_tac[trans_com_choice_r,trans_par_r,qcong_par,qcong_refl])
+      >- (fs[endpoints_def,ALL_DISTINCT_APPEND] >>
+          qpat_x_assum `_ _ LTau _` assume_tac >>
+          drule endpoint_local_confluence_int_choice >>
+          disch_then drule >>
+          impl_tac >- (simp[] >> metis_tac[trans_distinct_residual,label_distinct,
+                                           label_rel_def,receive_ext_choice_rel_def,
+                                           choice_sender_is_endpoint,choice_receiver_is_endpoint]) >>
+          strip_tac >>
+          metis_tac[trans_com_choice_r,trans_par_r,qcong_par,qcong_refl])
+      >- (dxrule_then (qspec_then `p2` assume_tac) trans_par_l >>
+          asm_exists_tac >> simp[] >> pop_assum kall_tac >>
+          rename1 `NPar q` >>
+          dxrule_then (qspec_then `q` assume_tac) trans_par_r >>
+          asm_exists_tac >> simp[qcong_refl])
+      >- (dxrule_then (qspec_then `p2` assume_tac) trans_par_l >>
+          asm_exists_tac >> simp[] >> pop_assum kall_tac >>
+          rename1 `NPar q` >>
+          dxrule_then (qspec_then `q` assume_tac) trans_par_r >>
+          asm_exists_tac >> simp[qcong_refl])
+      >- (fs[endpoints_def,ALL_DISTINCT_APPEND] >>
+          first_x_assum(drule_all_then strip_assume_tac) >>
+          imp_res_tac trans_par_r >>
+          rpt(first_x_assum(qspec_then `n1` assume_tac)) >>
+          ntac 2 (asm_exists_tac >> simp[]) >>
+          metis_tac[qcong_rules]))
+QED
+
+(* TODO: move? *)
+Theorem REPLICATE_SUC_SNOC:
+  REPLICATE (SUC m) e = REPLICATE m e ++ [e]
+Proof
+  simp[REPLICATE_GENLIST] >>
+  match_mp_tac LIST_EQ >>
+  rw[EL_CONS_IF] >>
+  rw[EL_APPEND_EQN] >>
+  `x - m = 0` by intLib.COOPER_TAC >>
+  simp[]
+QED
+
+Theorem endpoint_confluence_contract:
+  ∀m p1 p2 p3.
+   trans p1 LTau p2 /\
+   list_trans p1 (REPLICATE m LTau) p3 /\
+   ALL_DISTINCT (MAP FST (endpoints p1))
+   ==>
+   (?n p4. list_trans p2 (REPLICATE n LTau) p4 /\
+        n <= m /\
+        qcong p3 p4) \/
+   (?n p4 p5. list_trans p2 (REPLICATE n LTau) p4 /\
+        trans p3 LTau p5 /\
+        n <= m /\
+        qcong p4 p5)
+Proof
+  Induct >> rpt strip_tac
+  >- (fs[list_trans_def] >> rveq >>
+      disj2_tac >> asm_exists_tac >> simp[qcong_refl])
+  >> FULL_SIMP_TAC bool_ss [REPLICATE_SUC_SNOC]
+  >> fs[list_trans_append,list_trans_def]
+  >> first_x_assum drule_all
+  >> strip_tac
+  >- (drule qcong_trans_pres >>
+      disch_then drule >> strip_tac >>
+      `list_trans p2 (REPLICATE (SUC n) LTau) q2`
+        by(PURE_REWRITE_TAC[REPLICATE_SUC_SNOC] >>
+           rw[list_trans_append,list_trans_def] >>
+           metis_tac[]) >>
+      disj1_tac >>
+      asm_exists_tac >> simp[])
+  >- (Cases_on `p3 = p5`
+      >- (rveq >>
+          disj1_tac >> asm_exists_tac >>
+          simp[qcong_sym]) >>
+      disj2_tac >>
+      imp_res_tac endpoint_names_trans >>
+      imp_res_tac endpoint_names_list_trans >>      
+      dxrule endpoint_local_confluence_tau >>
+      disch_then dxrule >>
+      impl_tac >- simp[] >>
+      strip_tac >>
+      qhdtm_x_assum `qcong` mp_tac >>
+      drule_all(qcong_trans_pres |> PURE_ONCE_REWRITE_RULE [qcong_sym_eq]) >>
+      rpt strip_tac >>
+      `list_trans p2 (REPLICATE (SUC n) LTau) q2`
+        by(PURE_ONCE_REWRITE_TAC [REPLICATE_SUC_SNOC] >>
+           rw[list_trans_def,list_trans_append] >> metis_tac[]) >>
+      asm_exists_tac >> simp[] >>
+      asm_exists_tac >> simp[] >>
+      metis_tac[qcong_trans])
+QED
+
+Theorem endpoint_confluence_weak_contract:
+  ∀n m p1 p2 p3.
+   list_trans p1 (REPLICATE n LTau) p2 /\
+   list_trans p1 (REPLICATE m LTau) p3 /\
+   ALL_DISTINCT (MAP FST (endpoints p1))
+   ==>
+   (?n' m' p4 p5. list_trans p2 (REPLICATE n' LTau) p4 /\
+        list_trans p3 (REPLICATE m' LTau) p5 /\
+        n' <= m /\ m' <= n /\
+        qcong p4 p5)
+Proof
+  Induct >> rpt strip_tac
+  >- (fs[list_trans_def] >> rveq >>
+      asm_exists_tac >> simp[qcong_refl])
+  >> FULL_SIMP_TAC bool_ss [REPLICATE_SUC_SNOC]
+  >> fs[list_trans_append,list_trans_def]
+  >> first_x_assum drule_all
+  >> strip_tac
+  >> drule endpoint_confluence_contract
+  >> disch_then drule
+  >> impl_tac
+  >- (imp_res_tac endpoint_names_trans >>
+      imp_res_tac endpoint_names_list_trans >>
+      fs[])
+  >> strip_tac
+  >- (asm_exists_tac >> simp[] >> asm_exists_tac >> simp[] >> metis_tac[qcong_rules])
+  >> qhdtm_x_assum `qcong` mp_tac
+  >> drule qcong_trans_pres  
+  >> disch_then drule
+  >> strip_tac
+  >> `list_trans p3 (REPLICATE (SUC m') LTau) q2` (* TODO: (mild) generated names *)
+        by(PURE_REWRITE_TAC[REPLICATE_SUC_SNOC] >>
+           rw[list_trans_append,list_trans_def] >>
+           metis_tac[])
+  >> strip_tac
+  >> asm_exists_tac >> simp[]
+  >> asm_exists_tac >> simp[]
+  >> metis_tac[qcong_rules]
+QED
+
+val _ = export_theory();
